Messing with modules for PtoI / ItoP and provenance.
I think I need to be able to do these kinds of things in order to
define concretizations with UVALUE_ExtractBytes / UVALUE_ConcatBytes.

In particular, concretization of ConcatBytes in the non-trivial cases
involves actually extracting a byte value from each of the uvalue
bytes. It makes sense to do this for the integer that corresponds to a
pointer, so I need ptr_to_int for this.

Similarly, if I have a list of bytes that is being deserialized into a
ptr, I need to be able to use int_to_ptr. int_to_ptr may also involve
a provenance.

src/coq/Handlers/Serialization.v
@@ -7,12 +7,14 @@ From Vellvm Require Import
      Utils.Error
      Utils.ListUtil
      Utils.NonEmpty
+     Utils.NMaps
      Syntax.LLVMAst
      Syntax.DynamicTypes
      Syntax.DataLayout
      Semantics.DynamicValues
      Semantics.Denotation
      Semantics.MemoryAddress
+     Semantics.Memory.Sizeof
      Semantics.LLVMEvents.
 
 From ExtLib Require Import
@@ -26,13 +28,37 @@ Require Import Lia.
 Import ListNotations.
 Import MonadNotation.
 
-Module Make(LLVMEvents: LLVM_INTERACTIONS(Addr)).
-  Import LLVMEvents.
+(* TODO: move this? *)
+Module Type PTOI(Addr:MemoryAddress.ADDRESS).  
+  Parameter ptr_to_int : Addr.addr -> Z.
+End PTOI.
+
+(* TODO: move this? *)
+Module Type PROVENANCE(Addr:MemoryAddress.ADDRESS).
+  Parameter Prov : Set.
+  Parameter wildcard_prov : Prov.
+  Parameter nil_prov : Prov.
+  Parameter address_provenance : Addr.addr -> Prov.
+End PROVENANCE.
+
+(* TODO: move this? *)
+Module Type ITOP(Addr:MemoryAddress.ADDRESS)(PROV:PROVENANCE(Addr)).
+  Parameter int_to_ptr : Z -> PROV.Prov -> Addr.addr.
+End ITOP.
+
+Module Make(Addr:MemoryAddress.ADDRESS)(LLVMIO: LLVM_INTERACTIONS(Addr))(SIZEOF: Sizeof)(PTOI:PTOI(Addr))(PROVENANCE:PROVENANCE(Addr))(ITOP:ITOP(Addr)(PROVENANCE)).
+
+  Import LLVMIO.
+  Import SIZEOF.
+  Import PTOI.
+  Import PROVENANCE.
+  Import ITOP.
   Import DV.
   Open Scope list.
 
   Definition addr := Addr.addr.
 
+  (* TODO: move this? *)
   Inductive SByte :=
   | UByte (uv : uvalue) (dt : dtyp) (idx : uvalue) (sid : store_id) : SByte.
 
@@ -107,6 +133,30 @@ Module Make(LLVMEvents: LLVM_INTERACTIONS(Addr)).
          | UByte uv dt idx sid => UVALUE_ExtractByte uv dt idx sid
          end.
 
+    (* Is a uvalue a concrete integer equal to i? *)
+    Definition uvalue_int_eq_Z (uv : uvalue) (i : Z)
+      := match uv with
+         | UVALUE_I1 x
+         | UVALUE_I8 x
+         | UVALUE_I32 x
+         | UVALUE_I64 x => Z.eqb (unsigned x) i
+         | UVALUE_IPTR x => Z.eqb x i
+         | _ => false
+         end.
+
+    Definition dvalue_int_unsigned (dv : dvalue) : Z
+      := match dv with
+         | DVALUE_I1 x => unsigned x
+         | DVALUE_I8 x => unsigned x
+         | DVALUE_I32 x => unsigned x
+         | DVALUE_I64 x => unsigned x
+         | DVALUE_IPTR x => x (* TODO: unsigned???? *)
+         | _ => 0
+         end.
+
+    Definition guard_opt (x : bool) : option unit
+      := if x then Some tt else None.
+
     Fixpoint all_bytes_from_uvalue_helper (idx' : Z) (sid' : store_id) (parent : uvalue) (bytes : list SByte) : option uvalue
       := match bytes with
          | [] => Some parent
@@ -122,6 +172,35 @@ Module Make(LLVMEvents: LLVM_INTERACTIONS(Addr)).
          | nil => None
          | cons (UByte uv dt idx sid) xs =>
            all_bytes_from_uvalue_helper 0 sid uv bytes
+         end.
+
+    (* TODO: move this *)
+    Definition dtyp_eqb (dt1 dt2 : dtyp) : bool
+      := match @dtyp_eq_dec dt1 dt2 with
+         | left x => true
+         | right x => false
+         end.
+
+    Fixpoint all_extract_bytes_from_uvalue_helper (idx' : Z) (sid' : store_id) (dt' : dtyp) (parent : uvalue) (bytes : list uvalue) : option uvalue
+      := match bytes with
+         | [] => Some parent
+         | (UVALUE_ExtractByte uv dt idx sid)::bytes =>
+           guard_opt (uvalue_int_eq_Z idx idx');;
+           guard_opt (RelDec.rel_dec uv parent);;
+           guard_opt (N.eqb sid sid');;
+           guard_opt (dtyp_eqb dt dt');;
+           all_extract_bytes_from_uvalue_helper (Z.succ idx') sid' dt' parent bytes
+         | _ => None
+         end.
+
+    (* Check that store ids, uvalues, and types match up, as well as
+       that the extract byte indices are in the right order *)
+    Definition all_extract_bytes_from_uvalue (bytes : list uvalue) : option uvalue
+      := match bytes with
+         | nil => None
+         | (UVALUE_ExtractByte uv dt idx sid)::xs =>
+           all_extract_bytes_from_uvalue_helper 0 sid dt uv bytes
+         | _ => None
          end.
 
     Definition from_ubytes (bytes : list SByte) (dt : dtyp) : uvalue
@@ -271,6 +350,17 @@ Module Make(LLVMEvents: LLVM_INTERACTIONS(Addr)).
 
     Definition filter_sid_matches (byte : SByte) (sbytes : list (N * SByte)) : (list (N * SByte) * list (N * SByte))
       := filter_split (fun '(n, uv) => sbyte_sid_match byte uv) sbytes.
+
+    (* TODO: move to some utility file? *)
+    Fixpoint NM_find_many {A} (xs : list N) (nm : NMap A) : option (list A)
+      := match xs with
+         | [] => ret []
+         | (x::xs) =>
+           elt  <- NM.find x nm;;
+           elts <- NM_find_many xs nm;;
+           ret (elt :: elts)
+         end.
+
 
     (* Assign fresh sids to ubytes while preserving entanglement *)
     Unset Guard Checking.
@@ -589,7 +679,177 @@ Module Make(LLVMEvents: LLVM_INTERACTIONS(Addr)).
 
        *)
 
+      (* TODO: probably move this *)
+      (* TODO: Make these take endianess into account.
+
+         Can probably use bitwidth from VInt to do big-endian...
+       *)
+      Definition extract_byte_vint {I} `{VInt I} (i : I) (idx : Z) : Z
+        := unsigned (modu (shru i (repr (idx * 8))) (repr 256)).
+
+      Fixpoint concat_bytes_vint {I} `{VInt I} (bytes : list I) : I
+        := match bytes with
+           | [] => repr 0
+           | (byte::bytes) =>
+             add byte (shl (concat_bytes_vint bytes) (repr 8))
+           end.
+
+      (* TODO: Endianess *)
+      (* TODO: does this work correctly with negative x? *)
+      Definition extract_byte_Z (x : Z) (idx : Z) : Z
+        := (Z.shiftr x (idx * 8)) mod 256.
+
+      (* TODO: Endianess *)
+      Definition concat_bytes_Z_vint {I} `{VInt I} (bytes : list Z) : I
+        := concat_bytes_vint (map repr bytes).
+
+      (* TODO: Endianess *)
+      Fixpoint concat_bytes_Z (bytes : list Z) : Z
+        := match bytes with
+           | [] => 0
+           | (byte::bytes) =>
+             byte + (Z.shiftl (concat_bytes_Z bytes) 8)
+           end.
+
+      (* TODO: Move this? *)
+      Inductive Poisonable (A : Type) : Type :=
+      | Unpoisoned : A -> Poisonable A
+      | Poison : Poisonable A
+      .
+
+      Arguments Unpoisoned {A} a.
+      Arguments Poison {A}.
+
+      Global Instance MonadPoisonable : Monad Poisonable
+        := { ret  := @Unpoisoned;
+             bind := fun _ _ ma mab => match ma with
+                                   | Poison => Poison
+                                   | Unpoisoned v => mab v
+                                    end
+           }.
+
+      Definition ErrPoison := eitherT string Poisonable.
+
+      (* Walk through a list *)
+      (* Returns field index + number of bytes remaining *)
+      Fixpoint extract_field_byte_helper {M} `{Monad M} (fields : list dtyp) (field_idx : N) (byte_idx : N) : eitherT string M (dtyp * (N * N))
+        := match fields with
+           | [] =>
+             raise "No fields left for byte-indexing..."
+           | (x::xs) =>
+             let sz := sizeof_dtyp x
+             in if N.ltb byte_idx sz
+                then ret (x, (field_idx, byte_idx))
+                else extract_field_byte_helper xs (N.succ field_idx) (byte_idx - sz)
+           end.
+
+      Fixpoint extract_field_byte {M} `{Monad M} (fields : list dtyp) (byte_idx : N) : eitherT string M (dtyp * (N * N))
+        := extract_field_byte_helper fields 0 byte_idx.
       
+      (* Need the type of the dvalue in order to know how big fields and array elements are.
+
+         It's not possible to use the dvalue alone, as DVALUE_Poison's
+         size depends on the type.
+       *)
+      (* TODO: make termination checker happy *)
+      Unset Guard Checking.
+      Fixpoint dvalue_extract_byte (dv : dvalue) (dt : dtyp) (idx : Z) {struct dv}: ErrPoison Z
+        := match dv with
+           | DVALUE_I1 x
+           | DVALUE_I8 x
+           | DVALUE_I32 x
+           | DVALUE_I64 x =>
+             ret (extract_byte_vint x idx)
+           | DVALUE_IPTR x =>
+             ret (extract_byte_Z x idx)
+           | DVALUE_Addr addr =>
+             (* Note: this throws away provenance *)
+             ret (extract_byte_Z (ptr_to_int addr) idx)
+           | DVALUE_Float f =>
+             ret (extract_byte_Z (unsigned (Float32.to_bits f)) idx)
+           | DVALUE_Double d =>
+             ret (extract_byte_Z (unsigned (Float.to_bits d)) idx)
+           | DVALUE_Poison => lift Poison
+           | DVALUE_None =>
+             (* TODO: Not sure if this should be an error, poison, or what. *)
+             raise "dvalue_extract_byte on DVALUE_None"
+           (* TODO: Take padding into account. *)
+           | DVALUE_Struct fields =>
+             match dt with
+             | DTYPE_Struct dts =>
+               (* Step to field which contains the byte we want *)
+               '(fdt, (field_idx, byte_idx)) <- extract_field_byte dts (Z.to_N idx) ;;
+               match List.nth_error fields (N.to_nat field_idx) with
+               | Some f =>
+                 (* call dvalue_extract_byte recursively on the field *)
+                 dvalue_extract_byte f fdt (Z.of_N byte_idx)
+               | None =>
+                 raise "dvalue_extract_byte: more fields in dvalue than in dtyp."
+               end
+             | _ => raise "dvalue_extract_byte: type mismatch on DVALUE_Struct."
+             end
+           | DVALUE_Packed_struct fields =>
+             match dt with
+             | DTYPE_Packed_struct dts =>
+               (* Step to field which contains the byte we want *)
+               '(fdt, (field_idx, byte_idx)) <- extract_field_byte dts (Z.to_N idx) ;;
+               match List.nth_error fields (N.to_nat field_idx) with
+               | Some f =>
+                 (* call dvalue_extract_byte recursively on the field *)
+                 dvalue_extract_byte f fdt (Z.of_N byte_idx)
+               | None =>
+                 raise "dvalue_extract_byte: more fields in dvalue than in dtyp."
+               end
+             | _ => raise "dvalue_extract_byte: type mismatch on DVALUE_Packed_struct."
+             end
+           | DVALUE_Array elts =>
+             match dt with
+             | DTYPE_Array sz dt =>
+               let elmt_sz  := sizeof_dtyp dt in
+               let elmt_idx := N.div (Z.to_N idx) elmt_sz in
+               let byte_idx := (Z.to_N idx) mod elmt_sz in
+               match List.nth_error elts (N.to_nat elmt_idx) with
+               | Some elmt =>
+                 (* call dvalue_extract_byte recursively on the field *)
+                 dvalue_extract_byte elmt dt (Z.of_N byte_idx)
+               | None =>
+                 raise "dvalue_extract_byte: more fields in dvalue than in dtyp."
+               end
+             | _ =>
+               raise "dvalue_extract_byte: type mismatch on DVALUE_Array."
+             end
+           | DVALUE_Vector elts =>
+             match dt with
+             | DTYPE_Vector sz dt =>
+               let elmt_sz  := sizeof_dtyp dt in
+               let elmt_idx := N.div (Z.to_N idx) elmt_sz in
+               let byte_idx := (Z.to_N idx) mod elmt_sz in
+               match List.nth_error elts (N.to_nat elmt_idx) with
+               | Some elmt =>
+                 (* call dvalue_extract_byte recursively on the field *)
+                 dvalue_extract_byte elmt dt (Z.of_N byte_idx)
+               | None =>
+                 raise "dvalue_extract_byte: more fields in dvalue than in dtyp."
+               end
+             | _ =>
+               raise "dvalue_extract_byte: type mismatch on DVALUE_Vector."
+             end
+           end.
+      Set Guard Checking.
+
+      (* Taking a byte out of a dvalue...
+
+      Unlike UVALUE_ExtractByte, I don't think this needs an sid
+      (store id). There should be no nondeterminism in this value. *)
+      Inductive dvalue_byte : Type :=
+      | DVALUE_ExtractByte (dv : dvalue) (dt : dtyp) (idx : N) : dvalue_byte
+      .
+
+      Definition dvalue_byte_value (db : dvalue_byte) : ErrPoison Z
+        := match db with
+           | DVALUE_ExtractByte dv dt idx =>
+             dvalue_extract_byte dv dt (Z.of_N idx)
+           end.
 
       (* TODO: probably satisfy the termination checker with length of xs... *)
       Unset Guard Checking.
@@ -600,6 +860,109 @@ Module Make(LLVMEvents: LLVM_INTERACTIONS(Addr)).
              take n xs :: split_every n (drop n xs)
            end.
       Set Guard Checking.
+
+      Unset Guard Checking.
+      Fixpoint dvalue_bytes_to_dvalue (dbs : list dvalue_byte) (dt : dtyp) {struct dt} : ErrPoison dvalue
+        := match dt with
+           | DTYPE_I sz =>
+             zs <- map_monad dvalue_byte_value dbs;;
+             match sz with
+             | 1 =>
+               ret (DVALUE_I1 (concat_bytes_Z_vint zs))
+             | 8 =>
+               ret (DVALUE_I8 (concat_bytes_Z_vint zs))
+             | 32 =>
+               ret (DVALUE_I32 (concat_bytes_Z_vint zs))
+             | 64 =>
+               ret (DVALUE_I64 (concat_bytes_Z_vint zs))
+             | _ => raise "Unsupported integer size."
+             end
+           | DTYPE_IPTR =>
+             zs <- map_monad dvalue_byte_value dbs;;
+             ret (DVALUE_IPTR (concat_bytes_Z zs))
+           | DTYPE_Pointer =>
+             (* TODO: not sure if this should be wildcard provenance.
+                TODO: not sure if this should truncate iptr value...
+              *)
+             zs <- map_monad dvalue_byte_value dbs;;
+             ret (DVALUE_Addr (int_to_ptr (concat_bytes_Z zs) wildcard_prov))
+           | DTYPE_Void =>
+             raise "dvalue_bytes_to_dvalue on void type."
+           | DTYPE_Half =>
+             raise "dvalue_bytes_to_dvalue: unsupported DTYPE_Half."
+           | DTYPE_Float =>
+             zs <- map_monad dvalue_byte_value dbs;;
+             ret (DVALUE_Float (Float32.of_bits (concat_bytes_Z_vint zs)))
+           | DTYPE_Double =>
+             zs <- map_monad dvalue_byte_value dbs;;
+             ret (DVALUE_Float (Float32.of_bits (concat_bytes_Z_vint zs)))
+           | DTYPE_X86_fp80 =>
+             raise "dvalue_bytes_to_dvalue: unsupported DTYPE_X86_fp80."
+           | DTYPE_Fp128 =>
+             raise "dvalue_bytes_to_dvalue: unsupported DTYPE_Fp128."
+           | DTYPE_Ppc_fp128 =>
+             raise "dvalue_bytes_to_dvalue: unsupported DTYPE_Ppc_fp128."
+           | DTYPE_Metadata =>
+             raise "dvalue_bytes_to_dvalue: unsupported DTYPE_Metadata."
+           | DTYPE_X86_mmx =>
+             raise "dvalue_bytes_to_dvalue: unsupported DTYPE_X86_mmx."
+           | DTYPE_Array sz t =>
+             let sz := sizeof_dtyp t in
+             let elt_bytes := split_every sz dbs in
+             elts <- map_monad (fun es => dvalue_bytes_to_dvalue es t) elt_bytes;;
+             ret (DVALUE_Array elts)
+           | DTYPE_Vector sz t =>
+             let sz := sizeof_dtyp t in
+             let elt_bytes := split_every sz dbs in
+             elts <- map_monad (fun es => dvalue_bytes_to_dvalue es t) elt_bytes;;
+             ret (DVALUE_Vector elts)
+           | DTYPE_Struct fields =>
+             match fields with
+             | [] => ret (DVALUE_Struct []) (* TODO: Not 100% sure about this. *)
+             | (dt::dts) =>
+               let sz := sizeof_dtyp dt in
+               let init_bytes := take sz dbs in
+               let rest_bytes := drop sz dbs in
+               f <- dvalue_bytes_to_dvalue init_bytes dt;;
+               rest <- dvalue_bytes_to_dvalue rest_bytes (DTYPE_Struct dts);;
+               match rest with
+               | DVALUE_Struct fs =>
+                 ret (DVALUE_Struct (f::fs))
+               | _ =>
+                 raise "dvalue_bytes_to_dvalue: DTYPE_Struct recursive call did not return a struct."
+               end
+             end
+           | DTYPE_Packed_struct fields =>
+             match fields with
+             | [] => ret (DVALUE_Packed_struct []) (* TODO: Not 100% sure about this. *)
+             | (dt::dts) =>
+               let sz := sizeof_dtyp dt in
+               let init_bytes := take sz dbs in
+               let rest_bytes := drop sz dbs in
+               f <- dvalue_bytes_to_dvalue init_bytes dt;;
+               rest <- dvalue_bytes_to_dvalue rest_bytes (DTYPE_Struct dts);;
+               match rest with
+               | DVALUE_Packed_struct fs =>
+                 ret (DVALUE_Packed_struct (f::fs))
+               | _ =>
+                 raise "dvalue_bytes_to_dvalue: DTYPE_Packed_struct recursive call did not return a struct."
+               end
+             end
+           | DTYPE_Opaque =>
+             raise "dvalue_bytes_to_dvalue: unsupported DTYPE_Opaque."
+           end.
+      Set Guard Checking.
+
+      Definition uvalue_sid_match (a b : uvalue) : bool
+        :=
+          match a, b with
+          | UVALUE_ExtractByte uv dt idx sid, UVALUE_ExtractByte uv' dt' idx' sid' =>
+            RelDec.rel_dec uv uv' && N.eqb sid sid'
+          | _, _ => false
+          end.
+
+      Definition filter_uvalue_sid_matches (byte : uvalue) (uvs : list (N * uvalue)) : (list (N * uvalue) * list (N * uvalue))
+        := filter_split (fun '(n, uv) => uvalue_sid_match byte uv) uvs.
 
 
       Definition ErrPoison_to_undef_or_err_dvalue (ep : ErrPoison dvalue) : undef_or_err dvalue
@@ -904,146 +1267,146 @@ Section ConcretizeInd.
   Variable endianess : Endianess.
 
   (* TODO: probably move this *)
-  Inductive concretize_u : uvalue -> undef_or_err dvalue -> Prop :=
-  (* TODO: should uvalue_to_dvalue be modified to handle concatbytes? *)
-  (* Concrete uvalue are concretized into their singleton *)
-  | Pick_concrete             : forall uv (dv : dvalue), uvalue_to_dvalue uv = inr dv -> concretize_u uv (ret dv)
-  | Pick_fail                 : forall uv v s, ~ (uvalue_to_dvalue uv = inr v)  -> concretize_u uv (lift (failwith s))
-  (* Undef relates to all dvalue of the type *)
-  | Concretize_Undef          : forall dt dv,
-      dvalue_has_dtyp dv dt ->
-      concretize_u (UVALUE_Undef dt) (ret dv)
+  (* Inductive concretize_u : uvalue -> undef_or_err dvalue -> Prop := *)
+  (* (* TODO: should uvalue_to_dvalue be modified to handle concatbytes? *) *)
+  (* (* Concrete uvalue are concretized into their singleton *) *)
+  (* | Pick_concrete             : forall uv (dv : dvalue), uvalue_to_dvalue uv = inr dv -> concretize_u uv (ret dv) *)
+  (* | Pick_fail                 : forall uv v s, ~ (uvalue_to_dvalue uv = inr v)  -> concretize_u uv (lift (failwith s)) *)
+  (* (* Undef relates to all dvalue of the type *) *)
+  (* | Concretize_Undef          : forall dt dv, *)
+  (*     dvalue_has_dtyp dv dt -> *)
+  (*     concretize_u (UVALUE_Undef dt) (ret dv) *)
 
-  (* The other operations proceed non-deterministically *)
-  | Concretize_IBinop : forall iop uv1 e1 uv2 e2,
-      concretize_u uv1 e1 ->
-      concretize_u uv2 e2 ->
-      concretize_u (UVALUE_IBinop iop uv1 uv2)
-                   (dv1 <- e1 ;;
-                    dv2 <- e2 ;;
-                    (eval_iop iop dv1 dv2))
+  (* (* The other operations proceed non-deterministically *) *)
+  (* | Concretize_IBinop : forall iop uv1 e1 uv2 e2, *)
+  (*     concretize_u uv1 e1 -> *)
+  (*     concretize_u uv2 e2 -> *)
+  (*     concretize_u (UVALUE_IBinop iop uv1 uv2) *)
+  (*                  (dv1 <- e1 ;; *)
+  (*                   dv2 <- e2 ;; *)
+  (*                   (eval_iop iop dv1 dv2)) *)
                    
-  | Concretize_ICmp : forall cmp uv1 e1 uv2 e2 ,
-      concretize_u uv1 e1 ->
-      concretize_u uv2 e2 ->
-      concretize_u (UVALUE_ICmp cmp uv1 uv2)
-                   (dv1 <- e1 ;;
-                    dv2 <- e2 ;;
-                    eval_icmp cmp dv1 dv2)
+  (* | Concretize_ICmp : forall cmp uv1 e1 uv2 e2 , *)
+  (*     concretize_u uv1 e1 -> *)
+  (*     concretize_u uv2 e2 -> *)
+  (*     concretize_u (UVALUE_ICmp cmp uv1 uv2) *)
+  (*                  (dv1 <- e1 ;; *)
+  (*                   dv2 <- e2 ;; *)
+  (*                   eval_icmp cmp dv1 dv2) *)
 
-  | Concretize_FBinop : forall fop fm uv1 e1 uv2 e2,
-      concretize_u uv1 e1 ->
-      concretize_u uv2 e2 ->
-      concretize_u (UVALUE_FBinop fop fm uv1 uv2)
-                   (dv1 <- e1 ;;
-                    dv2 <- e2 ;;
-                    eval_fop fop dv1 dv2)
+  (* | Concretize_FBinop : forall fop fm uv1 e1 uv2 e2, *)
+  (*     concretize_u uv1 e1 -> *)
+  (*     concretize_u uv2 e2 -> *)
+  (*     concretize_u (UVALUE_FBinop fop fm uv1 uv2) *)
+  (*                  (dv1 <- e1 ;; *)
+  (*                   dv2 <- e2 ;; *)
+  (*                   eval_fop fop dv1 dv2) *)
 
-  | Concretize_FCmp : forall cmp uv1 e1 uv2 e2,
-      concretize_u uv1 e1 ->
-      concretize_u uv2 e2 ->
-      concretize_u (UVALUE_FCmp cmp uv1 uv2)
-                   (dv1 <- e1 ;;
-                    dv2 <- e2 ;;
-                    eval_fcmp cmp dv1 dv2)
+  (* | Concretize_FCmp : forall cmp uv1 e1 uv2 e2, *)
+  (*     concretize_u uv1 e1 -> *)
+  (*     concretize_u uv2 e2 -> *)
+  (*     concretize_u (UVALUE_FCmp cmp uv1 uv2) *)
+  (*                  (dv1 <- e1 ;; *)
+  (*                   dv2 <- e2 ;; *)
+  (*                   eval_fcmp cmp dv1 dv2) *)
 
-  | Concretize_Struct_Nil     : concretize_u (UVALUE_Struct []) (ret (DVALUE_Struct []))
-  | Concretize_Struct_Cons    : forall u e us es,
-      concretize_u u e ->
-      concretize_u (UVALUE_Struct us) es ->
-      concretize_u (UVALUE_Struct (u :: us))
-                   (d <- e ;;
-                    vs <- es ;;
-                    match vs with
-                    | (DVALUE_Struct ds) => ret (DVALUE_Struct (d :: ds))
-                    | _ => failwith "illegal Struct Cons"
-                    end)
+  (* | Concretize_Struct_Nil     : concretize_u (UVALUE_Struct []) (ret (DVALUE_Struct [])) *)
+  (* | Concretize_Struct_Cons    : forall u e us es, *)
+  (*     concretize_u u e -> *)
+  (*     concretize_u (UVALUE_Struct us) es -> *)
+  (*     concretize_u (UVALUE_Struct (u :: us)) *)
+  (*                  (d <- e ;; *)
+  (*                   vs <- es ;; *)
+  (*                   match vs with *)
+  (*                   | (DVALUE_Struct ds) => ret (DVALUE_Struct (d :: ds)) *)
+  (*                   | _ => failwith "illegal Struct Cons" *)
+  (*                   end) *)
 
 
-  | Concretize_Packed_struct_Nil     : concretize_u (UVALUE_Packed_struct []) (ret (DVALUE_Packed_struct []))
-  | Concretize_Packed_struct_Cons    : forall u e us es,
-      concretize_u u e ->
-      concretize_u (UVALUE_Packed_struct us) es ->
-      concretize_u (UVALUE_Packed_struct (u :: us))
-                   (d <- e ;;
-                    vs <- es ;;
-                    match vs with
-                    | (DVALUE_Packed_struct ds) => ret (DVALUE_Packed_struct (d :: ds))
-                    | _ => failwith "illegal Packed_struct cons"
-                    end)
+  (* | Concretize_Packed_struct_Nil     : concretize_u (UVALUE_Packed_struct []) (ret (DVALUE_Packed_struct [])) *)
+  (* | Concretize_Packed_struct_Cons    : forall u e us es, *)
+  (*     concretize_u u e -> *)
+  (*     concretize_u (UVALUE_Packed_struct us) es -> *)
+  (*     concretize_u (UVALUE_Packed_struct (u :: us)) *)
+  (*                  (d <- e ;; *)
+  (*                   vs <- es ;; *)
+  (*                   match vs with *)
+  (*                   | (DVALUE_Packed_struct ds) => ret (DVALUE_Packed_struct (d :: ds)) *)
+  (*                   | _ => failwith "illegal Packed_struct cons" *)
+  (*                   end) *)
 
-  | Concretize_Array_Nil :
-      concretize_u (UVALUE_Array []) (ret (DVALUE_Array []))
+  (* | Concretize_Array_Nil : *)
+  (*     concretize_u (UVALUE_Array []) (ret (DVALUE_Array [])) *)
 
-  | Concretize_Array_Cons : forall u e us es,
-      concretize_u u e ->
-      concretize_u (UVALUE_Array us) es ->
-      concretize_u (UVALUE_Array (u :: us))
-                   (d <- e ;;
-                    vs <- es ;;
-                    match vs with
-                    | (DVALUE_Array ds) => ret (DVALUE_Array (d :: ds))
-                    | _ => failwith "illegal Array cons"
-                    end)
+  (* | Concretize_Array_Cons : forall u e us es, *)
+  (*     concretize_u u e -> *)
+  (*     concretize_u (UVALUE_Array us) es -> *)
+  (*     concretize_u (UVALUE_Array (u :: us)) *)
+  (*                  (d <- e ;; *)
+  (*                   vs <- es ;; *)
+  (*                   match vs with *)
+  (*                   | (DVALUE_Array ds) => ret (DVALUE_Array (d :: ds)) *)
+  (*                   | _ => failwith "illegal Array cons" *)
+  (*                   end) *)
 
-  | Concretize_Vector_Nil :
-      concretize_u (UVALUE_Vector []) (ret (DVALUE_Vector []))
+  (* | Concretize_Vector_Nil : *)
+  (*     concretize_u (UVALUE_Vector []) (ret (DVALUE_Vector [])) *)
 
-  | Concretize_Vector_Cons : forall u e us es,
-      concretize_u u e ->
-      concretize_u (UVALUE_Vector us) es ->
-      concretize_u (UVALUE_Vector (u :: us))
-                   (d <- e ;;
-                    vs <- es ;;
-                    match vs with
-                    | (DVALUE_Vector ds) => ret (DVALUE_Vector (d :: ds))
-                    | _ => failwith "illegal Vector cons"
-                    end)
+  (* | Concretize_Vector_Cons : forall u e us es, *)
+  (*     concretize_u u e -> *)
+  (*     concretize_u (UVALUE_Vector us) es -> *)
+  (*     concretize_u (UVALUE_Vector (u :: us)) *)
+  (*                  (d <- e ;; *)
+  (*                   vs <- es ;; *)
+  (*                   match vs with *)
+  (*                   | (DVALUE_Vector ds) => ret (DVALUE_Vector (d :: ds)) *)
+  (*                   | _ => failwith "illegal Vector cons" *)
+  (*                   end) *)
 
-  | Concretize_ConcatBytes_Int :
-      forall bytes sz,
-        (forall byte, In byte bytes -> exists idx, byte = UVALUE_ExtractByte byte idx)
-          concretize_u (UVALUE_ConcatBytes bytes (DTYPE_I sz))
-          _
-  .
+  (* | Concretize_ConcatBytes_Int : *)
+  (*     forall bytes sz, *)
+  (*       (forall byte, In byte bytes -> exists idx, byte = UVALUE_ExtractByte byte idx) *)
+  (*         concretize_u (UVALUE_ConcatBytes bytes (DTYPE_I sz)) *)
+  (*         _ *)
+  (* . *)
 
-  (* The thing that's bothering me... *)
+  (* (* The thing that's bothering me... *) *)
 
-  (*      Converting to DVALUE destroys information... *)
+  (* (*      Converting to DVALUE destroys information... *) *)
 
-  (*      Maybe it doesn't matter, though... *)
+  (* (*      Maybe it doesn't matter, though... *) *)
 
-  (*    *)
+  (* (*    *) *)
 
-  (* May not concretize to anything. Should be a type error *)
-  | Concretize_ExtractByte :
-      forall byte idx c_byte c_idx,
-        concretize_u byte c_byte ->
-        concretize_u idx  c_idx ->
-        concretize_u (UVALUE_ExtractByte byte idx)
-                     (c_byte' <- c_byte;;
-                      c_idx'  <- c_idx;;
-                      match c_byte' with
-                      | DVALUE_Addr a => _
-                      | DVALUE_I1 x => _
-                      | DVALUE_I8 x => _
-                      | DVALUE_I32 x => _
-                      | DVALUE_I64 x => _
-                      | DVALUE_IPTR x => _
-                      | DVALUE_Double x => _
-                      | DVALUE_Float x => _
-                      | DVALUE_Poison => _
-                      | DVALUE_None => _
-                      | DVALUE_Struct fields => _
-                      | DVALUE_Packed_struct fields => _
-                      | DVALUE_Array elts => _
-                      | DVALUE_Vector elts => _
-                      end
-                     )
-  | Concretize_ConcatBytes_Int :
-      forall bytes sz,
-        concretize_u (UVALUE_ConcatBytes bytes (DTYPE_I sz))
-                     (ret DVALUE_None)
-  .
+  (* (* May not concretize to anything. Should be a type error *) *)
+  (* | Concretize_ExtractByte : *)
+  (*     forall byte idx c_byte c_idx, *)
+  (*       concretize_u byte c_byte -> *)
+  (*       concretize_u idx  c_idx -> *)
+  (*       concretize_u (UVALUE_ExtractByte byte idx) *)
+  (*                    (c_byte' <- c_byte;; *)
+  (*                     c_idx'  <- c_idx;; *)
+  (*                     match c_byte' with *)
+  (*                     | DVALUE_Addr a => _ *)
+  (*                     | DVALUE_I1 x => _ *)
+  (*                     | DVALUE_I8 x => _ *)
+  (*                     | DVALUE_I32 x => _ *)
+  (*                     | DVALUE_I64 x => _ *)
+  (*                     | DVALUE_IPTR x => _ *)
+  (*                     | DVALUE_Double x => _ *)
+  (*                     | DVALUE_Float x => _ *)
+  (*                     | DVALUE_Poison => _ *)
+  (*                     | DVALUE_None => _ *)
+  (*                     | DVALUE_Struct fields => _ *)
+  (*                     | DVALUE_Packed_struct fields => _ *)
+  (*                     | DVALUE_Array elts => _ *)
+  (*                     | DVALUE_Vector elts => _ *)
+  (*                     end *)
+  (*                    ) *)
+  (* | Concretize_ConcatBytes_Int : *)
+  (*     forall bytes sz, *)
+  (*       concretize_u (UVALUE_ConcatBytes bytes (DTYPE_I sz)) *)
+  (*                    (ret DVALUE_None) *)
+  (* . *)
 
-  Definition concretize (uv: uvalue) (dv : dvalue) := concretize_u uv (ret dv).
+  (* Definition concretize (uv: uvalue) (dv : dvalue) := concretize_u uv (ret dv). *)
